*Notes 2019-09-18*

\textbf{Definition.} We say the integer $a$ is invertible modulo $m$ if there exists $b\in\mathbb Z$ s.t. $ab \equiv 1 \pmod m$.

$$ab \equiv 1 \pmod m \Leftrightarrow \bar a \cdot \bar b = \bar 1$$ where $b$ is an inverse of $a$ and $\bar b$ is an inverse of $\bar a$

**Observation**: if $a$ is invertible modulo $m$, then all integers in the residue class are invertible modulo $m$. 

This is because $a\cdot b \equiv 1 \pmod m \Rightarrow (a + k \cdot m) \cdot b \equiv 1\pmod m$ and $ab + kbm \equiv 1 + 0 \equiv 1 \pmod m$

**Ex**. 3 is invertible modulo 7 because $3 \times 5 \equiv 1 \pmod 7$

Assume $b$ and $c$ are inverses of $a$. So $a\cdot b \equiv a\cdot c \equiv 1 \pmod m$. Proof: $abc \equiv c \pmod m \Rightarrow (ac) b \equiv c \pmod m \Rightarrow b \equiv c \mod m$.

**Proposition**: $a\in\mathbb Z$ is invertible modulo $m$ $\Leftrightarrow \gcd(a, m) = 1$.

*Proof*: $(\Leftarrow)$ Assume $\gcd(a, m) = 1$. Then $ax + my = \gcd(a, m)$ for some integers $x, y$. So therefore $ax \equiv 1 \pmod m$.

$(\Rightarrow)$ Assume $\exists b \in \mathbb Z$ s.t. $ab \equiv 1 \pmod m$. Let $d = \gcd(a, m)$. So $d|a \Rightarrow d|ab$ and $d|m \Rightarrow d|mk$. So $d|(ab - mk) \Rightarrow d|1$. Hence $\gcd(a, m) = 1$. \qedsymbol

**Definition** $\{\bar i : 0 \leq i \leq m - 1, \gcd(i, m) \equiv 1\} =: (\mathbb Z /m\mathbb Z)^*$

**Motivation**: Given $m\in\mathbb Z \setminus \{0\}$ and $f\in \mathbb Z[x]$, we want to solve $f(x) \equiv 0 \pmod m$ for $x\in\mathbb Z$.

**Proposition**. Let $f\in\mathbb Z[x]$ and $m\in\mathbb Z\setminus\{0\}$, and let $a, b\in\mathbb Z$ s.t. $a\equiv b \pmod m$. Then $f(a) \equiv f(b) \pmod m$.

Idea: Try $x\in \{0,\ldots m - 1\}$ and see whether $f(x) \equiv 0 \pmod m$. If $f(j) \equiv 0 \pmod m$ and $j \in\{0,\ldots m- 1\}$, then $f(j + km) \equiv 0 \pmod m$.

Notice: $f\in\mathbb Z[X] \Rightarrow \bar f \in \mathbb Z/m\mathbb Z[X] \Rightarrow \bar f(\bar x) = \bar 0$.

*Proof* (prop): write $f(x) = c_0 + c_1x + \ldots + c_nx^n$ where $c_1 \in \mathbb Z$. We desire  $c_0 + c_1a + \ldots c_na^n \equiv c_0 + c_1b + \ldots c_nb^n \pmod m$. Each term on the left is congruent to the associated term on the right because $a \equiv b \Rightarrow a^n \equiv b^n \pmod m$. \qedsymbol

**Proposition**: $$ax \equiv ay \pmod m \Leftrightarrow x \equiv y \pmod {\frac m{\gcd (a, m)}}$$

*Proof*: Let $d = \gcd(a, m)$ and $a_1 = \frac ad$, $m_1 = \frac md \in \mathbb Z$.

$(\Leftarrow)$ if $x \equiv y \pmod {m_1}$ then $dx \equiv dy \pmod {dm_1 = m}$.

So, $dx \equiv dy \pmod m$, so $a_1 dx \equiv a_1 dy \pmod m$ and so $ax \equiv ay \pmod m$.
