*Notes 2019-10-23*

**Theorem**: let $p$ be an odd prime. Let $\alpha \in \mathbb N$. Then $\exists$ primitive root modulo $p^\alpha$. [*Ed.* That is, $\exists$ an element whose order is $\phi(p^\alpha)$.]

**Proof**: First consider $\alpha = 2$. We search for a primitive root modulo $p^2$ of the form $g_2 = g + p\ell$.

$\ord_p(g_2) = \ord_p(g) = p - 1$.

$ord_{p^2}(g_2) = k \Rightarrow g_2^k \equiv 1 \pmod(p^2)$

$\Rightarrow$ $g_2^k \equiv 1 \pmod p \Rightarrow p - 1 | k = \ord_{p^2}(g_2)$

$\ord_{p^2}(g_2) = k \Rightarrow k | \phi(p^2) = p(p-1)$

**Goal**: $k = p(p-1)$. So we argue either $p|k$ or $k \not = p-1$. We prove $k \not = p - 1$ (equiv. to $g_2^{p-1} \not \equiv  1 \pmod {p^2}$.

Recall: $g_2= g + p\ell$, so $\ell \in \{0,\ldots p-1\}$. [*Ed.* We're trying to construct $g_2$, so we get to choose $\ell$.]

Want: $g_2^{p-1} \not \equiv 1 \pmod {p^2}$.

\begin{align*}
&(g + \ell p)^{p-1} \not \equiv 1 \pmod {p^2}\\
\Leftrightarrow& g^p + \sum_{i=1}^p {p \choose i} g^{p - i}(\ell p)^i \not \equiv g + \ell p \pmod{p^2}\\
\Leftrightarrow& g^{p} \not \equiv g + \ell p \pmod{p^2}\\
\Leftrightarrow& g^p - g \not \equiv \ell p \pmod{p^2}
\end{align*}

We can pick some $\ell$ to make this work. Example: $g^p - g \not \equiv 0$ or $g^2 - g \not \equiv p$; whatever works. $\qed$

*Aside*: $\exists \ell$ s.t. $g^p - g \equiv \ell p \pmod {p^2}$ because $g^p - g \equiv 0 \pmod p$, so $p | g^p - g$.

\hrulefill

We move on to $\alpha > 2$ (induction on $\alpha$).

Assume $\ord_{p^\alpha}(g_2) \equiv p^{\alpha-1}(p-1)$ and we prove that $\ord_{p^{\alpha + 1}}(g_2) = p^\alpha(p-1)$
$[\alpha \geq 2]$ 

Let $k = \ord_{p^{\alpha + 1}}(g_2) | p^{\alpha}(p - 1)$

$g_2^k \equiv 1 \pmod {p^{\alpha + 1}} \Rightarrow g_2^k \equiv 1 \pmod {p^\alpha}$

But $\ord_{p^\alpha}(g_2) = p^{\alpha - 1}(p-1) \Rightarrow p^{\alpha - 1}(p - 1)|k|p^{\alpha}(p - 1)$

$k \not = p^{\alpha - 1}(p-1) \Leftrightarrow g_2^{p^{\alpha - 1}(p - 1)} \not\equiv 1 \pmod {p^{\alpha + 1}}$

$\Leftrightarrow$ We know (I.H) that $\ord_{p^\alpha}(p_2) = p^{\alpha - 1} (p-1) \not = p^{\alpha - 2}(p - 1)$

$\Leftrightarrow$ $g_2^{p^{\alpha - 2}(p-1)} \not \equiv 1 \pmod{p^\alpha}$

So $g_2^{p^{\alpha - 2}(p-1)}\not\equiv 1 \pmod {p^{\alpha}}$ (because root primitive)

*but* $g_2^{p^{\alpha - 2}(p-1)} \equiv 1 \pmod {p^{\alpha - 1}}$

$\Rightarrow$ $g_2^{p^{\alpha - 1}(p-1)} = 1 + p^{\alpha - 1}\ell$ and $p \not | \ell$
where $g_2^{p^{\alpha - 1}(p-1)} \equiv (g_2^{p^{\alpha - 2}(p - 1)})^p \equiv (1 + p^{\alpha - 1}\ell)^p \pmod {p^{\alpha + 2}}$

$\equiv 1 + {P \choose 1}p^{\alpha - 1}\ell + \sum_{i=2}^p (p^{\alpha - 1}\ell)^i$

$p^{\alpha + 1} | (p^{\alpha - 1}\ell)^i$ for $i \geq 2$

${p \choose 1}p^{\alpha - 1}\ell \equiv p^{\alpha}\ell \not \equiv 0 \pmod{p^{\alpha + 1}}$ since $p \not | \;\ell$.

$2 \leq i \leq p - 1$, $\exp_{p}({p \choose i}(p^{\alpha - 1}\ell)^i) = 1 + i\alpha - 1 \geq \alpha + 1$ (since $\alpha \geq 2$)

if $i = p$ then $\exp_{p}({p \choose p} (p^{\alpha - 1}\ell)^p) = (\alpha - 1)p \geq \alpha$ since $\alpha \geq 2, p > 2$. (Note: things break for $p = 2$). \qed
