*Notes 2019-10-09*

First, some playing around before we get to Hensel's lemma

$X^2 + X + 1 \equiv 0 \pmod 7$ (we'll call this $f(x)$.

$X_1 \equiv 2,4 \pmod 7$

What about $X^2 + X + 1 \equiv 0 \pmod{7^2}$ (Consider just solution $x=2$ for now; we're ignoring $x=4$).

Must have $x_2 \equiv 2 + 7\ell$, $0 \leq \ell \leq 6$; so our options are $2, 9, 16, 23, 30, 37, 44$

$$(2+7\ell)^2 + (2+7\ell) + 1 \equiv 0 \pmod {7^2}$$

$$(2^2 + 2 + 1 + 7\ell(2\cdot 2 + 1 + (7\ell)^2 \equiv 0 \pmod{7^2}$$

Note the first parenthesis here is $f(2)$, the second parenthesis is $f'(2)$

$$7 + 7\ell \cdot 5 \equiv 0 \pmod{7^2} \Leftrightarrow 1 + 5\ell \equiv 0 \pmod 7 \Rightarrow \ell = 4\Rightarrow x_2 = 30$$.

We were able to lift a solution from *level 1* $\pmod 7$ into *level 2* $\pmod {7^2}$. Let's try lifting into ``level 3'' $\pmod {7^3}$.

Well:

$x_3 = 30 + 7^2\ell$ with $0 \leq \ell \leq 6$ (that's due to the $7^2$ coefficient on $\ell$), so our options are $30, 79, 128, 177, 226, 275, 324$. 

$$X^2 + X + 1 \equiv 0 \pmod {7^3}$$

$$(30 + 7^2\ell) + (30 + 7^2\ell) + 1 \equiv 0 \pmod {7^3}$$

$$(30^2 + 30 + 1) + 7^2\ell(2\cdot 30 + 1) + (7^2\ell)^2 \equiv 0 \pmod{7^3}$$

Note that the first parenthesis is $f(3)$, the second is $f'(30)$. 

Works out to $931 + 7^2\ell \cdot 61 \equiv 0 \pmod{7^3}$. Note that the $7^2|931$; in particular, $7^2\cdot 19 + 7^2\ell\cdot61 \equiv 0 \pmod{7^3}$. We can cancel $7^2$ throughout to get $19 + 61\ell \equiv 0 \pmod 7$. This reduces to $-2-2\ell \equiv 0 \pmod 7$. Solution is $\ell = 6$. Thus $x_3 = 30 + 49\cdot 6 = 324$.

To go onto level 4, consider all the ``lifts'' into level 4, i.e. $324 + 7^3\ell$ for $0 \leq \ell \leq 6$

Let's try to formulate this

**Hensel's Lemma**

$Let f\in\mathbb Z[X]$ and $P$ be a prime and let $x_1\in\mathbb Z$ s.t. $f(x_1)\equiv 0\pmod P$ and $f'(x_1) \equiv 0 \pmod P$ (the derivative of $f$), then for each $n\in\mathbb N$, there exists a unique (we won't prove uniqueness) $x_n \equiv \mathbb Z$ s.t. $f(x_n) \equiv 0 \pmod {P^n}$ and $x_n \equiv x_1 \pmod P$.

*Proof*: Let $f(x) = C_dx^d + \ldots + C_0$ (all integer coefficients). We proceed by induction (which seems inviting).

The case $n=1$ is known already. We assume $f(x_n) \equiv 0 \pmod{P^n}$ and $x_n\equiv x_1\pmod P$ and then lift $x_n$ to a solution $x_{n+1} = x_n + p^n\ell$ (with $0 \leq \ell < P$) $\Rightarrow X_{n+1} \equiv X_n \equiv X_1\pmod P$.

\begin{align*}
f(X_{n+1}) &= f(X_n + P^n\ell)\\
 &= \sum_{i=1}^d c_i(x_n+P^n\ell)^i\\
&= (\sum_{i=1}^d c_i x_n^i) + p^n\ell \sum_{i=1}^d ic_ix_n^{i-1} + \sum_{j=2}^d (P^n\ell)^j\cdot \sum_{i=j}^dc_ix_n^{i-j} i\choose j\\
&\equiv f(x_n) + p^n\ell f'(x_n) \pmod p^{n+1}
\end{align*}

We know $f(x_n) \equiv 0 \pmod {P^n} \Rightarrow \exists x\in\mathbb Z$ s.t. $f(x_n) \equiv P^n \cdot k$

$f(x_{n+1}) \equiv 0 \pmod P^{n+1} \Leftrightarrow P^nk + P^n\ell f'(X_n) \equiv 0 \pmod P^{n+1}$

$\Leftrightarrow k + \ell f'(x_n) \equiv 0 \pmod P$ so $\exists \ell \in\mathbb Z$ solution since $4f'(x_n) \not\equiv 0 \pmod p$

$x_n \equiv x_1 \pmod P\Rightarrow  f'(x_n) \equiv f'(X_1) \not \equiv 0 \pmod P$

**P-adic norm**: For $x,y\in\mathbb Z$, we set $|x-y|_P = P^{-\exp_{p}(x-y)}$, where $\exp_P(x-y)$ is the exponent of $P$ in the prime factorization of $(x-y)$

In the $P$-adic norm, the difference between the solutions go to 0, so $x_\infty$ is a solution to $f(x)$ in $Z_P$.
